Reimplemented up to update_field_x but blocking

ulib/experimental/Steel.ArrayStruct.fst
@@ -24,7 +24,7 @@ open FStar.FunctionalExtensionality
 open Steel.PCM
 module PCMBase = Steel.PCM.Base
 
-open Steel.Effect.Fake
+open Steel.Effect
 open Steel.Memory
 
 let extract_update: unit -> Tot unit = (fun () -> ())
@@ -34,177 +34,102 @@ let extract_recombine: unit -> Tot unit = (fun () -> ())
 let op_String_Access : unit -> Tot unit = (fun () -> ())
 let generic_index: unit -> Tot unit = (fun () -> ())
 
-assume val h_admit (#a:Type) (#p:slprop) (#q:a -> slprop) (_:unit) : SteelT a p q
-
 #set-options "--fuel 0 --ifuel 1"
 
-let update_x (r: ref (option u32_pair) u32_pair_pcm) (new_val: UInt32.t)
-    : Steel unit (ptr r) (fun _ -> ptr r)
-    (fun h0 -> if Some? (sel r h0) then True else False) (fun h0 _ h1 ->
-     Some? (sel r h1) /\ Some? (sel r h0) /\
-     Some?.v (sel r h1) == { Some?.v (sel r h0) with x = new_val }
-    )
+let update_x
+  (r: ref (option u32_pair) u32_pair_pcm)
+  (old_pair: Ghost.erased u32_pair)
+  (new_val: UInt32.t)
+    : SteelT unit
+      (pts_to r (Some (Ghost.reveal old_pair)))
+      (fun _ -> pts_to r (Some ({ old_pair with x = new_val})))
   =
-  let old_pair = read r in
-  let new_pair = (Some ({Some?.v old_pair with x = new_val })) in
-  write r new_pair
+  let real_old_pair =  read r (Some (Ghost.reveal old_pair)) in
+  let new_pair = (Some ({Some?.v real_old_pair with x = new_val })) in
+  write r (Some (Ghost.reveal old_pair)) new_pair
 
-
-let get_x (r: ref (option u32_pair) u32_pair_pcm)
-  : Steel UInt32.t
-  (ptr r) (fun _ -> ptr r)
-  (fun h0 -> Some? (sel r h0)) (fun h0 v h1 ->
-    Some? (sel r h0) /\ Some? (sel r h1) /\
-    sel r h0 == sel r h1 /\ v == (Some?.v (sel r h1)).x
-  )
+let get_x
+  (r: ref (option u32_pair) u32_pair_pcm)
+  (pair: Ghost.erased u32_pair)
+    : SteelT (x:UInt32.t{pair.x == x})
+      (pts_to r (Some (Ghost.reveal pair)))
+      (fun x -> (pts_to r (Some (Ghost.reveal pair))))
   =
-  let pair = read r in
-  (Some?.v pair).x
+  let real_pair = read r (Some (Ghost.reveal pair)) in
+  (Some?.v real_pair).x
 
-
-let increment_generic (#cls: rw_pointer UInt32.t) (r: cls.pointer_ref) : Steel unit
-  (cls.pointer_slref r) (fun _ -> cls.pointer_slref r)
-  (fun h0 -> UInt32.v (cls.pointer_sel r h0) + 1 <= UInt.max_int 32)
-  (fun h0 _ h1 ->
-    UInt32.v (cls.pointer_sel r h1) == UInt32.v (cls.pointer_sel r h0) + 1
-  )
+let increment_generic
+  (#cls: rw_pointer UInt32.t)
+  (r: cls.pointer_ref)
+  (v: Ghost.erased UInt32.t{UInt32.v v + 1 <= UInt.max_int 32})
+    : SteelT unit
+      (cls.pointer_slref r v)
+      (fun _ -> cls.pointer_slref r (UInt32.add v 1ul))
   =
-  let old_v = cls.pointer_get r in
-  cls.pointer_upd r (UInt32.add old_v 1ul)
+  let old_v = cls.pointer_get r v in
+  cls.pointer_upd r v (UInt32.add old_v 1ul)
 
-let slu32_pair_elim_mem (r: u32_pair_ref) (h: hmem (slu32_pair r)) :
-  Lemma (interp (ptr r) h /\ begin let v = sel r h in
-    Some? v /\ snd (Some?.v v) == Full
-  end)
-  =
-  elim_h_exists
-    (fun (v: u32_pair_stored) -> pts_to r v `star` pure (Some? v /\ snd (Some?.v v) == Full))
-    h
-    (interp (ptr r) h /\ begin let v = sel r h in
-      Some? v /\ snd (Some?.v v) == Full
-    end)
-    (fun v ->
-      intro_h_exists v (pts_to r) h;
-      pure_interp (Some? v /\ snd (Some?.v v) == Full) h;
-      assert(interp (pure (Some? v /\ snd (Some?.v v) == Full)) h);
-      assert(Some? v /\ snd (Some?.v v) == Full);
-      let v' = sel_v r v h in
-      assert(v' == v)
-    )
+let u32_pair_get : rw_pointer_get_sig u32_pair u32_pair_ref slu32_pair =
+  fun r g_pair ->
+    let Some (Full pair) = read r (Some (Full (Ghost.reveal g_pair))) in
+    pair
 
-assume val slu32_pair_elim_steel (r: u32_pair_ref) : Steel unit
-  (slu32_pair r)
-  (fun _ -> ptr r)
-  (fun _ -> True)
-  (fun h0 _ h1 ->
-    slu32_pair_elim_mem r h0;
-    let v = sel r h0 in
-    Some? v /\ snd (Some?.v v) == Full /\
-    v == sel r h1
-  )
-
-assume val slu32_pair_intro_steel (r: u32_pair_ref) : Steel unit
-  (ptr r)
-  (fun _ -> slu32_pair r)
-  (fun h0 -> let v = sel r h0 in
-    Some? v /\ snd (Some?.v v) == Full
-  )
-  (fun h0 _ h1 ->
-    slu32_pair_elim_mem r h1;
-    sel r h0 == sel r h1
-  )
-
-let u32_pair_get : rw_pointer_get_sig u32_pair u32_pair_ref slu32_pair u32_pair_sel =
-  fun r ->
-    slu32_pair_elim_steel r;
-    let pair = read r in
-    slu32_pair_intro_steel r;
-    fst (Some?.v pair)
-
-let u32_pair_upd: rw_pointer_upd_sig u32_pair u32_pair_ref slu32_pair u32_pair_sel =
-  fun r v ->
-    slu32_pair_elim_steel r;
-    let pair = read r in
-    write r (Some (v, snd (Some?.v pair)));
-    slu32_pair_intro_steel r
-
-let slu32_pair_x_field_elim_mem (r: u32_pair_x_field_ref) (h: hmem (slu32_pair_x_field r)) :
-  Lemma (interp (ptr r) h /\ begin let v = sel r h in
-    Some? v /\ (snd (Some?.v v) == XField \/ snd (Some?.v v) == Full)
-  end)
-  =
-  elim_h_exists
-    (fun (v: u32_pair_stored) ->
-      pts_to r v `star` pure (Some? v /\ (snd (Some?.v v) == XField \/ snd (Some?.v v) == Full))
-    )
-    h
-    (interp (ptr r) h /\ begin let v = sel r h in
-      Some? v /\ (snd (Some?.v v) == XField \/ snd (Some?.v v) == Full)
-    end)
-    (fun v ->
-      intro_h_exists v (pts_to r) h;
-      pure_interp (Some? v /\ (snd (Some?.v v) == XField \/ snd (Some?.v v) == Full)) h;
-      let v' = sel_v r v h in
-      ()
-    )
-
-assume val slu32_pair_x_field_elim_steel (r: u32_pair_ref) : Steel unit
-  (slu32_pair_x_field r)
-  (fun _ -> ptr r)
-  (fun _ -> True)
-  (fun h0 _ h1 ->
-    slu32_pair_x_field_elim_mem r h0;
-    let v = sel r h0 in
-    Some? v /\ (snd (Some?.v v) == XField \/ snd (Some?.v v) == Full) /\
-    v == sel r h1
-  )
-
-assume val slu32_pair_x_field_intro_steel (r: u32_pair_ref) : Steel unit
-  (ptr r)
-  (fun _ -> slu32_pair_x_field r)
-  (fun h0 -> let v = sel r h0 in
-    Some? v /\ (snd (Some?.v v) == XField \/ snd (Some?.v v) == Full)
-  )
-  (fun h0 _ h1 ->
-    slu32_pair_x_field_elim_mem r h1;
-    sel r h0 == sel r h1
-  )
+let u32_pair_upd: rw_pointer_upd_sig u32_pair u32_pair_ref slu32_pair =
+  fun r g_pair v ->
+    let Some (Full pair) = read r (Some (Full (Ghost.reveal g_pair))) in
+    write r (Some (Full (Ghost.reveal g_pair))) (Some (Full v))
 
 let u32_pair_x_field_get
-  : rw_pointer_get_sig UInt32.t u32_pair_x_field_ref slu32_pair_x_field u32_pair_x_field_sel
+  : rw_pointer_get_sig UInt32.t u32_pair_x_field_ref slu32_pair_x_field
   =
-  fun r ->
-    slu32_pair_x_field_elim_steel r;
-    let pair = read r in
-    slu32_pair_x_field_intro_steel r;
-    (fst (Some?.v pair)).x
+  fun r g_x ->
+    match read r (Some (XField g_x)) with
+    | Some (XField x) -> x
+    | Some (Full pair) -> pair.x
 
+#push-options "--admit_smt_queries true"
 let u32_pair_x_field_upd
-  : rw_pointer_upd_sig UInt32.t u32_pair_x_field_ref slu32_pair_x_field u32_pair_x_field_sel
+  : rw_pointer_upd_sig UInt32.t u32_pair_x_field_ref slu32_pair_x_field
   =
-  fun r v ->
-    slu32_pair_x_field_elim_steel r;
-    let pair = read r in
-    let new_pair = (Some (({ fst (Some?.v pair) with x = v }), snd (Some?.v pair))) in
-    frame_preserving_intro u32_pair_stored_pcm pair new_pair
-      (fun frame -> ())
-      (fun frame ->
-        let p = snd (Some?.v pair) in
-        match p with
-        | XField -> begin match frame with
-          | None -> ()
-          | Some frame' -> begin match snd frame' with
-            | YField ->
-              let new_full = op u32_pair_stored_pcm frame new_pair in
-              let old_full = op u32_pair_stored_pcm frame pair in
-              assume(new_full == new_pair) // We don't have that because the path is Full in new_paip
-            | _ -> ()
-          end
-        end
-        | _ -> ()
-      );
-    assert(FStar.PCM.frame_preserving u32_pair_stored_pcm pair new_pair);
-    admit(); // Here the problem is that the write spec uses sel r h0 instead of pair, so we have
-             // to prove that because sel r h0 `compatible` pair, the frame preservation still holds
-    write r new_pair;
-    slu32_pair_x_field_intro_steel r
+  fun r g_x v ->
+   let new_val = match read r (Some (XField g_x)) with
+   | Some (XField x) -> Some (XField v)
+   | Some (Full pair) -> Some (Full ({pair with x = v}))
+   in
+   assert(FStar.PCM.frame_preserving u32_pair_stored_pcm (Some (XField g_x)) new_val);
+   write r (Some (XField g_x)) new_val
+#pop-options
+
+let u32_pair_y_field_get
+  : rw_pointer_get_sig UInt32.t u32_pair_y_field_ref slu32_pair_y_field
+  =
+  admit()
+
+let u32_pair_y_field_upd
+  : rw_pointer_upd_sig UInt32.t u32_pair_y_field_ref slu32_pair_y_field
+  =
+  admit()
+
+let recombinable (r: u32_pair_ref) (r12: u32_pair_x_field_ref & u32_pair_y_field_ref) : prop
+  = admit()
+
+let explose_u32_pair_into_x_y (r: u32_pair_ref) (pair: u32_pair)
+  : SteelT (r12:(u32_pair_x_field_ref & u32_pair_y_field_ref){recombinable r r12})
+  (slu32_pair r pair)
+  (fun (r1, r2) ->
+    slu32_pair_x_field r1 pair.x `star`
+    slu32_pair_y_field r2 pair.y)
+  =
+  Steel.SteelT.Basics.h_admit _ _
+
+let recombine_u32_pair_from_x_y
+  (r: u32_pair_ref)
+  (r1: u32_pair_x_field_ref)
+  (v1: UInt32.t)
+  (r2: u32_pair_y_field_ref)
+  (v2: UInt32.t)
+  : SteelT unit
+    (slu32_pair_x_field r1 v1 `star` slu32_pair_y_field r2 v2)
+    (fun _ -> slu32_pair r ({ x = v1; y = v2}))
+  =
+  Steel.SteelT.Basics.h_admit _ _
